Switched to records and started proving some lemmas

mechanization/theories/Core/Syntactic/Syntax.v
@@ -1,123 +1,129 @@
+From Coq Require Import List.
 From McPTS.Core Require Import Base.
 From McPTS.Core.PTSSignature Require Import Signature.
 
-Module SyntaxFunctor (P : PtsSig).
-  Import P.
 
-  (* Expressions M,N,A,B *)
-  Inductive Exp : Type :=
-  | a_st : St -> Exp                                             (* s *)
-  | a_var : nat -> Exp                                            (* x_i *)
-  | a_pi : forall (s1 s2 s3 : St), Ru s1 s2 s3 -> Exp -> Exp -> Exp   (* Π_r A.B *)
-  | a_lam : Exp -> Exp                                           (* λM *)
-  | a_app : Exp -> Exp -> Exp                                    (* M N *)
-  | a_clo : Sub -> Exp -> Exp                                    (* [σ]M *)
+(* Expressions M,N,A,B *)
+Inductive Exp (S : PtsSig) : Type :=
+| a_st : St S -> Exp S                                                  (* s *)
+| a_var : nat -> Exp S                                                   (* x_i *)
+| a_pi : forall (s1 s2 s3 : St S), Ru S s1 s2 s3 -> Exp S -> Exp S -> Exp S   (* Π_r A.B *)
+| a_lam : Exp S -> Exp S                                                (* λM *)
+| a_app : Exp S -> Exp S -> Exp S                                       (* M N *)
+| a_clo : Sub S -> Exp S -> Exp S                                       (* [σ]M *)
 
-  (* Substitutions σ,τ*)
-  with Sub : Type :=
-  | a_id : Sub                                                   (* id *)
-  | a_wk : Sub                                                   (* wk *)
-  | a_empty : Sub                                                (* .. *)
-  | a_ext : Sub -> Exp -> Sub                                     (* σ, M *)
-  | a_comp : Sub -> Sub -> Sub.                                   (* σ ∘ τ *) 
+(* Substitutions σ,τ*)
+with Sub (S : PtsSig) : Type :=
+| a_id : Sub S                                                        (* id *)
+| a_wk : Sub S                                                        (* wk *)
+| a_empty : Sub S                                                     (* .. *)
+| a_ext : Sub S -> Exp S -> Sub S                                     (* σ, M *)
+| a_comp : Sub S -> Sub S -> Sub S                                    (* σ ∘ τ *) 
+.
 
-  (* Typ is syntactic sugar to help differentiate terms and types *)
-  Notation Typ := Exp.
+(* The signature needs to be passed as an extra argument to each constructor, but is inferrable *)
+Arguments a_st {_}.
+Arguments a_var {_}.
+Arguments a_pi {_}.
+Arguments a_lam {_}.
+Arguments a_app {_}.
+Arguments a_clo {_}.
 
-  (* Contexts Γ,Δ *)
-  (*
-   *  I originally want to define Ctx as (list (Typ * St)).
-   *  For some reason, whenever I use this Ctx, Coq complains that ""Typ" has type "Type" while it is expected to have type "nat""
-   *  Defining it directly as an inductive type fixes the issue, but will it cause problems later on?
-   *)
-  Inductive Ctx : Type :=
-  | a_nil : Ctx
-  | a_cons : Ctx -> Exp -> St -> Ctx.
-
-  Fixpoint length (Γ : Ctx) : nat :=
-    match Γ with
-    | a_nil => 0
-    | a_cons Γ _ _ => S (length Γ)
-    end.
-
-  (* Notation Ctx := (list (Typ * St)). *)
-  
-
-  (* Neutral forms E *)
-  Inductive Ne : Type :=
-  | ne_var : nat -> Ne                                             (* x_i *)
-  | ne_app : Ne -> Nf -> Ne                                       (* E V *)
-                         
-  (* Normal forms V *)
-  with Nf : Type :=
-  | nf_ne : Ne -> Nf                                              (* E *)
-  | nf_st : St -> Nf                                              (* s *)
-  | nf_pi : forall (s1 s2 s3 : St), Ru s1 s2 s3 -> Nf -> Nf -> Nf       (* Π_r V1.V2 *)
-  | nf_lam : Nf -> Nf.                                            (* λV *)
+Arguments a_id {_}.
+Arguments a_wk {_}.
+Arguments a_empty {_}.
+Arguments a_ext {_}.
+Arguments a_comp {_}.
 
 
-  (* Coercion of neutral and normal forms into expressions.  Basically identity functions *)
-  Fixpoint Ne_to_Exp (E : Ne) : Exp :=
-    match E with
-    | ne_var i => a_var i
-    | ne_app E' V => a_app (Ne_to_Exp E') (Nf_to_Exp V)
-    end
-  with Nf_to_Exp (V : Nf) : Exp :=
-    match V with
-    | nf_ne E => Ne_to_Exp E
-    | nf_st s => a_st s
-    | nf_pi s1 s2 s3 r V1 V2 => a_pi s1 s2 s3 r (Nf_to_Exp V1) (Nf_to_Exp V2)
-    | nf_lam V => a_lam (Nf_to_Exp V)
-    end.
-
-  Coercion Nf_to_Exp : Nf >-> Exp.
-  Coercion Ne_to_Exp : Ne >-> Exp.
-
-  (* Convenient notation for writing expressions *)
-  (* #[global] Declare Custom Entry Exp. *)
-  (* #[global] Declare Custom Entry Nf. *)
-
-  #[global] Bind Scope mctt_scope with Exp.
-  #[global] Bind Scope mctt_scope with Sub.
-  #[global] Bind Scope mctt_scope with Nf.
-  #[global] Bind Scope mctt_scope with Ne.
-  Open Scope mctt_scope.
-
-  (* We need to define substitution notation first to assert [left associativity] of level 0. *)
-  Notation "[ σ ] e" := (a_clo σ e) (in custom Exp at level 0, e custom Exp, σ custom Exp at level 60, left associativity, format "[ σ ] e") : mctt_scope.
-  Notation "{{{ x }}}" := x (at level 0, x custom Exp at level 99, format "'{{{'  x  '}}}'") : mctt_scope.
-  Notation "( x )" := x (in custom Exp at level 0, x custom Exp at level 60) : mctt_scope.
-  Notation "'^' x" := x (in custom Exp at level 0, x constr at level 0) : mctt_scope.
-  Notation "x" := x (in custom Exp at level 0, x ident) : mctt_scope.
-
-  Notation "'Sort' @ s" := (a_st s) (in custom Exp at level 0, s constr at level 0, format "'Sort' @ s") : mctt_scope.
-  Notation "'#' i" := (a_var i) (in custom Exp at level 0, i constr at level 0, format "'#' i") : mctt_scope.  
-  Notation "'Π' r A B" := (a_pi _ _ _ r A B) (in custom Exp at level 1, r constr at level 0, A custom Exp at level 0, B custom Exp at level 60) : mctt_scope.
-  Notation "'λ' M" := (a_lam M) (in custom Exp at level 1, M custom Exp at level 60) : mctt_scope.
-  Notation "f x .. y" := (a_app .. (a_app f x) .. y) (in custom Exp at level 40, f custom Exp, x custom Exp at next level, y custom Exp at next level) : mctt_scope.
-
-  (* Notation for substitutions *)
-  Notation "'Id'" := a_id (in custom Exp at level 0) : mctt_scope.
-  Notation "'Wk'" := a_wk (in custom Exp at level 0) : mctt_scope.
-  Notation "'..'" := a_empty (in custom Exp at level 0) : mctt_scope.
-  Notation "σ ∘ τ" := (a_comp σ τ) (in custom Exp at level 40, right associativity, format "σ ∘ τ") : mctt_scope.
-  Notation "σ ,, e" := (a_ext σ e) (in custom Exp at level 50, left associativity, format "σ ,, e") : mctt_scope.
-
-  (* Notation for contexts *)
-  Notation "⋅" := (a_nil) (in custom Exp at level 0) : mctt_scope.
-  Notation "Γ , A : s" := (a_cons Γ A s) (in custom Exp at level 50, left associativity, format "Γ ,  A : s") : mctt_scope.
+Definition Typ (S : PtsSig) := Exp S.
+Definition Ctx (S : PtsSig) := list (Exp S * St S)%type.
 
 
-  (* Notation for normal and neutral forms *)
-  Notation "n{{{ x }}}" := x (at level 0, x custom Nf at level 99, format "'n{{{'  x  '}}}'") : mctt_scope.
-  Notation "( x )" := x (in custom Nf at level 0, x custom Nf at level 60) : mctt_scope.
-  Notation "'^' x" := x (in custom Nf at level 0, x constr at level 0) : mctt_scope.
-  Notation "x" := x (in custom Nf at level 0, x ident) : mctt_scope.
+(* Neutral forms E *)
+Inductive Ne (S : PtsSig) : Type :=
+| ne_var : nat -> Ne S                                                      (* x_i *) 
+| ne_app : Ne S -> Nf S -> Ne S                                            (* E V *)
+                       
+(* Normal forms V *)
+with Nf (S : PtsSig) : Type :=
+| nf_ne : Ne S -> Nf S                                                     (* E *)
+| nf_st : St S -> Nf S                                                     (* s *)
+| nf_pi : forall (s1 s2 s3 : St S), Ru S s1 s2 s3 -> Nf S -> Nf S -> Nf S       (* Π_r V1.V2 *)
+| nf_lam : Nf S -> Nf S                                                  (* λV *)
+.
 
-  Notation "'Sort' @ s" := (nf_st s) (in custom Nf at level 0, s constr at level 0, format "'Sort' @ s") : mctt_scope.
-  Notation "'Π' r V1 V2" := (nf_pi _ _ _ r V1 V2) (in custom Nf at level 2, V1 custom Nf at level 1, V2 custom Nf at level 60) : mctt_scope.
-  Notation "'λ' V" := (nf_lam V) (in custom Nf at level 2, V custom Nf at level 60) : mctt_scope.
-  Notation "f x .. y" := (ne_app .. (ne_app f x) .. y) (in custom Nf at level 40, f custom Nf, x custom Nf at next level, y custom Nf at next level) : mctt_scope.
-  Notation "'#' i" := (ne_var i) (in custom Nf at level 0, i constr at level 0, format "'#' i") : mctt_scope.
-  Notation "'⇑' E" := (nf_ne E) (in custom Nf at level 0, E custom Nf at level 99, format "'⇑'  E") : mctt_scope.
-End SyntaxFunctor.
+Arguments ne_var {_}.
+Arguments ne_app {_}.
+
+Arguments nf_ne {_}.
+Arguments nf_st {_}.
+Arguments nf_pi {_}.
+Arguments nf_lam {_}.
+
+
+(* Coercion of neutral and normal forms into expressions.  Basically identity functions *)
+Fixpoint Ne_to_Exp (S : PtsSig) (E : Ne S) : Exp S :=
+  match E with
+  | ne_var i => a_var i
+  | ne_app E' V => a_app (Ne_to_Exp S E') (Nf_to_Exp S V)
+  end
+with Nf_to_Exp (S : PtsSig) (V : Nf S) : Exp S :=
+       match V with
+       | nf_ne E => Ne_to_Exp S E
+       | nf_st s => a_st s
+       | nf_pi s1 s2 s3 r V1 V2 => a_pi s1 s2 s3 r (Nf_to_Exp S V1) (Nf_to_Exp S V2)
+       | nf_lam V => a_lam (Nf_to_Exp S V)
+       end.
+
+Coercion Nf_to_Exp : Nf >-> Exp.
+Coercion Ne_to_Exp : Ne >-> Exp.
+
+
+(* Convenient notation for writing expressions *)
+#[global] Declare Custom Entry Exp.
+#[global] Declare Custom Entry Nf.
+
+#[global] Bind Scope mcpts_scope with Exp.
+#[global] Bind Scope mcpts_scope with Sub.
+#[global] Bind Scope mcpts_scope with Nf.
+#[global] Bind Scope mcpts_scope with Ne.
+Open Scope mcpts_scope.
+
+(* We need to define substitution notation first to assert [left associativity] of level 0. *)
+Notation "[ σ ] e" := (a_clo σ e) (in custom Exp at level 0, e custom Exp, σ custom Exp at level 60, left associativity, format "[ σ ] e") : mcpts_scope.
+Notation "{{{ x }}}" := x (at level 0, x custom Exp at level 99, format "'{{{'  x  '}}}'") : mcpts_scope.
+Notation "( x )" := x (in custom Exp at level 0, x custom Exp at level 60) : mcpts_scope.
+Notation "'^' x" := x (in custom Exp at level 0, x constr at level 0) : mcpts_scope.
+Notation "x" := x (in custom Exp at level 0, x ident) : mcpts_scope.
+
+Notation "'Sort' @ s" := (a_st s) (in custom Exp at level 0, s constr at level 0, format "'Sort' @ s") : mcpts_scope.
+Notation "'#' i" := (a_var i) (in custom Exp at level 0, i constr at level 0, format "'#' i") : mcpts_scope.  
+Notation "'Π' r A B" := (a_pi _ _ _ r A B) (in custom Exp at level 1, r constr at level 0, A custom Exp at level 0, B custom Exp at level 60) : mcpts_scope.
+Notation "'λ' M" := (a_lam M) (in custom Exp at level 1, M custom Exp at level 60) : mcpts_scope.
+Notation "f x .. y" := (a_app .. (a_app f x) .. y) (in custom Exp at level 40, f custom Exp, x custom Exp at next level, y custom Exp at next level) : mcpts_scope.
+
+(* Notation for substitutions *)
+Notation "'Id'" := a_id (in custom Exp at level 0) : mcpts_scope.
+Notation "'Wk'" := a_wk (in custom Exp at level 0) : mcpts_scope.
+Notation "'..'" := a_empty (in custom Exp at level 0) : mcpts_scope.
+Notation "σ ∘ τ" := (a_comp σ τ) (in custom Exp at level 40, right associativity, format "σ ∘ τ") : mcpts_scope.
+Notation "σ ,, e" := (a_ext σ e) (in custom Exp at level 50, left associativity, format "σ ,, e") : mcpts_scope.
+
+(* Notation for contexts *)
+Notation "⋅" := (nil) (in custom Exp at level 0) : mcpts_scope.
+Notation "Γ , A : s" := (cons (A, s) Γ) (in custom Exp at level 50, left associativity, format "Γ ,  A : s") : mcpts_scope.
+
+
+(* Notation for normal and neutral forms *)
+Notation "n{{{ x }}}" := x (at level 0, x custom Nf at level 99, format "'n{{{'  x  '}}}'") : mcpts_scope.
+Notation "( x )" := x (in custom Nf at level 0, x custom Nf at level 60) : mcpts_scope.
+Notation "'^' x" := x (in custom Nf at level 0, x constr at level 0) : mcpts_scope.
+Notation "x" := x (in custom Nf at level 0, x ident) : mcpts_scope.
+
+Notation "'Sort' @ s" := (nf_st s) (in custom Nf at level 0, s constr at level 0, format "'Sort' @ s") : mcpts_scope.
+Notation "'Π' r V1 V2" := (nf_pi _ _ _ r V1 V2) (in custom Nf at level 2, V1 custom Nf at level 1, V2 custom Nf at level 60) : mcpts_scope.
+Notation "'λ' V" := (nf_lam V) (in custom Nf at level 2, V custom Nf at level 60) : mcpts_scope.
+Notation "f x .. y" := (ne_app .. (ne_app f x) .. y) (in custom Nf at level 40, f custom Nf, x custom Nf at next level, y custom Nf at next level) : mcpts_scope.
+Notation "'#' i" := (ne_var i) (in custom Nf at level 0, i constr at level 0, format "'#' i") : mcpts_scope.
+Notation "'⇑' E" := (nf_ne E) (in custom Nf at level 0, E custom Nf at level 99, format "'⇑'  E") : mcpts_scope.
