mechanization/theories/Core/PTSSignature/Predicativity.v
@@ -1,11 +1,11 @@
 From Coq Require Import Relation_Definitions RelationClasses.
 From McPTS.Core.PTSSignature Require Import Signature.
 
-Module Type PredicativeSig (S : PtsSig).
-  Import S.
 
-  Axiom predicative : exists (P : relation St),
-      order St P
-      /\ (forall (s1 : St) (s2 : St), Ax s1 s2 -> P s1 s2)
-      /\ (forall (s1 s2 s3 : St), Ru s1 s2 s3 -> (P s1 s3) /\ (P s2 s3)).
-End PredicativeSig.
+Record PredicativeSig (S : PtsSig) : Prop :=
+  mkPredicativeSig {
+      test : exists (P : relation (St S)),
+        order (St S) P
+        /\ (forall s1 s2 : St S, Ax S s1 s2 -> P s1 s2)
+        /\ (forall s1 s2 s3 : St S, Ru S s1 s2 s3 -> (P s1 s3) /\ (P s2 s3))
+    }.
