mechanization/theories/Core/Syntactic/System/Lemmas.v
@@ -1,38 +1,157 @@
+From McPTS Require Import LibTactics.
 From McPTS.Core Require Import Base.
 From McPTS.Core.PTSSignature Require Import Signature.
-From McPTS.Core.Syntactic Require Export Syntax.
 From McPTS.Core.Syntactic.System Require Import Definitions.
 
-Module SystemLemmaFunctor (P : PtsSig).
-  Module Syn := SyntaxFunctor P.  
-  Module Sys := SystemFunctor P.
-  
-  Import P Syn Sys.
-  
-  (* Basic context properties *)
-  Lemma ctx_lookup_lt : forall {Γ x A s},
+(* Basic properties of contexts *)
+Lemma ctx_lookup_lt {P : PtsSig} : forall {Γ : Ctx P} {x : nat} {A : Typ P} {s : St P},
       {{ #x : A : s ∈ Γ }} ->
       x < length Γ.
-  Proof.
-    induction 1; simpl; lia.
-  Qed.
-  #[export]
-    Hint Resolve ctx_lookup_lt : mctt.
+Proof.
+  induction 1; simpl; lia.
+Qed.
+#[export]
+  Hint Resolve ctx_lookup_lt : mcpts.
 
-  Lemma functional_ctx_lookup : forall {Γ A A' x},
-      {{ #x : A ∈ Γ }} ->
-      {{ #x : A' ∈ Γ }} ->
-      A = A'.
-  Proof with mautosolve.
-    intros * Hx Hx'; gen A'.
-    induction Hx as [|* ? IHHx]; intros; inversion_clear Hx';
-      f_equal;
-      intuition.
-  Qed.
 
-  Lemma ctx_decomp : forall {Γ A}, {{ ⊢ Γ, A }} -> {{ ⊢ Γ }} /\ exists i, {{ Γ ⊢ A : Type@i }}.
-  Proof with now eauto.
-    inversion 1...
-  Qed.
+Lemma functional_ctx_lookup {P : PtsSig} : forall {Γ : Ctx P} {x A A' s},
+    {{ #x : A : s ∈ Γ }} ->
+    {{ #x : A' : s ∈ Γ }} ->
+    A = A'.
+Proof with mautosolve.
+  intros * Hx Hx'; gen A'.
+  induction Hx as [|* ? IHHx]; intros; inversion_clear Hx';
+    f_equal;
+    intuition.
+Qed.
 
-End SystemLemma.
+
+Lemma ctx_decomp {P : PtsSig} : forall {Γ : Ctx P} {A s},
+    {{ ⊢ Γ, A : s}} -> {{ ⊢ Γ }} /\ exists i, {{ Γ ⊢ A : Sort@i }}.
+Proof with now eauto.
+  inversion 1...
+Qed.
+
+#[export]
+  Hint Resolve ctx_decomp : mcpts.
+
+Corollary ctx_decomp_left {P : PtsSig} : forall {Γ : Ctx P} {A s}, {{ ⊢ Γ , A : s}} -> {{ ⊢ Γ }}.
+Proof with easy.
+  intros * ?%ctx_decomp...
+Qed.
+
+Corollary ctx_decomp_right {P : PtsSig} : forall {Γ : Ctx P} {A s}, {{ ⊢ Γ, A : s }} -> exists i, {{ Γ ⊢ A : Sort@i }}.
+Proof with easy.
+  intros * ?%ctx_decomp...
+Qed.
+
+#[export]
+Hint Resolve ctx_decomp_left ctx_decomp_right : mcpts.
+
+
+(** ** Core Presuppositions *)
+
+(** *** Context Presuppositions *)
+
+Lemma presup_ctx_eq {P : PtsSig} : forall {Γ Δ : Ctx P}, {{ ⊢ Γ ≡ Δ }} -> {{ ⊢ Γ }} /\ {{ ⊢ Δ }}.
+Proof with mautosolve.
+  induction 1; split; econstructor; destruct_pairs; assumption.
+Qed.
+
+Corollary presup_ctx_eq_left {P : PtsSig} : forall {Γ Δ : Ctx P}, {{ ⊢ Γ ≡ Δ }} -> {{ ⊢ Γ }}.
+Proof with easy.
+  intros * ?%presup_ctx_eq...
+Qed.
+
+Corollary presup_ctx_eq_right {P : PtsSig} : forall {Γ Δ : Ctx P}, {{ ⊢ Γ ≡ Δ }} -> {{ ⊢ Δ }}.
+Proof with easy.
+  intros * ?%presup_ctx_eq...
+Qed.
+
+#[export]
+Hint Resolve presup_ctx_eq presup_ctx_eq_left presup_ctx_eq_right : mcpts.
+
+Lemma presup_sub {P : PtsSig}: forall {Γ Δ : Ctx P} {σ}, {{ Γ ⊢s σ : Δ }} -> {{ ⊢ Γ }} /\ {{ ⊢ Δ }}.
+Proof with mautosolve.
+  induction 1; split; mauto; destruct_pairs; mauto; econstructor; assumption.
+Qed.
+
+Corollary presup_sub_left {P : PtsSig} : forall {Γ Δ : Ctx P} {σ}, {{ Γ ⊢s σ : Δ }} -> {{ ⊢ Γ }}.
+Proof with easy.
+  intros * ?%presup_sub...
+Qed.
+
+Corollary presup_sub_right {P : PtsSig} : forall {Γ Δ : Ctx P} {σ}, {{ Γ ⊢s σ : Δ }} -> {{ ⊢ Δ }}.
+Proof with easy.
+  intros * ?%presup_sub...
+Qed.
+
+#[export]
+Hint Resolve presup_sub presup_sub_left presup_sub_right : mcpts.
+
+(** With [presup_sub], we can prove similar for [exp]. *)
+
+Lemma presup_exp_ctx {P : PtsSig} : forall {Γ : Ctx P} {M A}, {{ Γ ⊢ M : A }} -> {{ ⊢ Γ }}.
+Proof with mautosolve.
+  induction 1...
+Qed.
+
+#[export]
+Hint Resolve presup_exp_ctx : mcpts.
+
+(** and other presuppositions about context well-formedness. *)
+
+Lemma presup_sub_eq_ctx {P : PtsSig} : forall {Γ Δ : Ctx P} {σ σ'}, {{ Γ ⊢s σ ≡ σ' : Δ }} -> {{ ⊢ Γ }} /\ {{ ⊢ Δ }}.
+Proof with mautosolve.
+  induction 1; split; mauto; try econstructor; mauto; destruct_pairs; mauto.
+Qed.
+
+Corollary presup_sub_eq_ctx_left {P : PtsSig} : forall {Γ Δ : Ctx P} {σ σ'}, {{ Γ ⊢s σ ≡ σ' : Δ }} -> {{ ⊢ Γ }}.
+Proof with easy.
+  intros * ?%presup_sub_eq_ctx...
+Qed.
+
+Corollary presup_sub_eq_ctx_right {P : PtsSig} : forall {Γ Δ : Ctx P} {σ σ'}, {{ Γ ⊢s σ ≡ σ' : Δ }} -> {{ ⊢ Δ }}.
+Proof with easy.
+  intros * ?%presup_sub_eq_ctx...
+Qed.
+
+#[export]
+Hint Resolve presup_sub_eq_ctx presup_sub_eq_ctx_left presup_sub_eq_ctx_right : mcpts.
+
+Lemma presup_exp_eq_ctx {P : PtsSig} : forall {Γ : Ctx P} {M M' A}, {{ Γ ⊢ M ≡ M' : A }} -> {{ ⊢ Γ }}.
+Proof with mautosolve 2.
+  induction 1...
+Qed.
+
+#[export]
+Hint Resolve presup_exp_eq_ctx : mcpts.
+
+(** *** Immediate Results of Context Presuppositions *)
+
+Lemma wf_conv {P : PtsSig} : forall (Γ : Ctx P) M A i A',
+    {{ Γ ⊢ M : A }} ->
+    (** The next argument will be removed in SystemOpt *)
+    {{ Γ ⊢ A' : Sort@i }} ->
+    {{ Γ ⊢ A ≡ A' : Sort@i }} ->
+    {{ Γ ⊢ M : A' }}.
+Proof.
+  intros.
+  econstructor; mauto.
+  econstructor; mauto.  
+Qed.
+
+#[export]
+Hint Resolve wf_conv : mcpts.
+
+Lemma wf_sub_conv {P : PtsSig} : forall (Γ : Ctx P) σ Δ Δ',
+  {{ Γ ⊢s σ : Δ }} ->
+  {{ ⊢ Δ ≡ Δ' }} ->
+  {{ Γ ⊢s σ : Δ' }}.
+Proof.
+  intros.
+  econstructor; mauto.
+Qed.
+
+#[export]
+Hint Resolve wf_sub_conv : mcpts.
