mechanization/theories/Core/Syntactic/System/Tactics.v
@@ -1,0 +1,80 @@
+From McPTS Require Import LibTactics.
+From McPTS.Core Require Import Base.
+From McPTS.Core.Syntactic.System Require Export Definitions Lemmas.
+
+#[global]
+Ltac pi_univ_level_tac :=
+  match goal with
+  | |- {{ ^_ ⊢s ^_ : ^_ }} => mauto 4
+  | H : {{ ^?Δ ⊢ ^?A : Sort@?j }} |- {{ ^?Δ , ^?A : ^?s ⊢ ^?B : Sort@?i }} =>
+      eapply lift_exp_max_right; mauto 4
+  | |- {{ ^?Δ ⊢ ^?A : Sort@?j }} =>
+      eapply lift_exp_max_left; mauto 4
+  end.
+
+#[export]
+Hint Rewrite -> wf_exp_eq_pi_sub using pi_univ_level_tac : mctt.
+
+#[local]
+Ltac invert_wf_ctx1 H :=
+  match type of H with
+  | {{ ⊢ ^?Γ, ^?A }} =>
+      let HΓ := fresh "HΓ" in
+      let HAi := fresh "HAi" in
+      pose proof ctx_decomp H as [HΓ HAi];
+      match goal with
+      | _: {{ Γ ⊢ A : Type@_ }} |- _ => clear HAi
+      | _: __mark__ _ {{ Γ ⊢ A : Type@_ }} |- _ => clear HAi
+      | _ =>
+          let i := fresh "i" in
+          let HA := fresh "HA" in
+          destruct HAi as [i HA]
+      end
+  end.
+
+Ltac invert_wf_ctx :=
+  (on_all_hyp: fun H => invert_wf_ctx1 H);
+  clear_dups.
+
+Ltac gen_core_presup H :=
+  match type of H with
+  | {{ ⊢ ^?Γ ≈ ^?Δ }} =>
+      let HΓ := fresh "HΓ" in
+      let HΔ := fresh "HΔ" in
+      pose proof presup_ctx_eq H as [HΓ HΔ]
+  | {{ ⊢ ^?Γ ⊆ ^?Δ }} =>
+      let HΓ := fresh "HΓ" in
+      let HΔ := fresh "HΔ" in
+      pose proof presup_ctx_sub H as [HΓ HΔ]
+  | {{ ^?Γ ⊢ ^?M : ^?A }} =>
+      let HΓ := fresh "HΓ" in
+      let HAi := fresh "HAi" in
+      pose proof presup_exp H as [HΓ HAi];
+      match goal with
+      | _: {{ Γ ⊢ A : Type@_ }} |- _ => clear HAi
+      | _: __mark__ _ {{ Γ ⊢ A : Type@_ }} |- _ => clear HAi
+      | _ =>
+          let i := fresh "i" in
+          let HA := fresh "HA" in
+          destruct HAi as [i HA]
+      end
+  | {{ ^?Γ ⊢s ^?σ : ^?Δ }} =>
+      let HΓ := fresh "HΓ" in
+      let HΔ := fresh "HΔ" in
+      pose proof presup_sub H as [HΓ HΔ]
+  end.
+
+Ltac gen_lookup_presup H :=
+  match type of H with
+  | {{ #?x : ^?A ∈ ^?Γ }} =>
+      match goal with
+      | _: {{ Γ ⊢ A : Type@_ }} |- _ => fail
+      | _: __mark__ _ {{ Γ ⊢ A : Type@_ }} |- _ => fail
+      | _ =>
+          let i := fresh "i" in
+          let HA := fresh "HA" in
+          pose proof presup_ctx_lookup_typ ltac:(eassumption) H as [i HA]
+      end
+  end.
+
+Ltac gen_core_presups := (on_all_hyp: fun H => gen_core_presup H); invert_wf_ctx; (on_all_hyp: fun H => gen_lookup_presup H); clear_dups.
