mechanization/theories/Core/Base.v
@@ -1,9 +1,7 @@
-#[global] Declare Scope mctt_scope.
-#[global] Delimit Scope mctt_scope with mctt.
-#[global] Bind Scope mctt_scope with Sortclass.
+#[global] Declare Scope mcpts_scope.
+#[global] Delimit Scope mcpts_scope with mcpts.
+#[global] Bind Scope mcpts_scope with Sortclass.
 
 #[global] Declare Custom Entry judg.
-#[global] Declare Custom Entry Exp.
-#[global] Declare Custom Entry Nf.
 
 Notation "{{ x }}" := x (at level 0, x custom judg at level 99, format "'{{'  x  '}}'").
